src/riot/RIoT.X509.AliasKeyTBS.Extensions.fst
@@ -3,10 +3,10 @@ module RIoT.X509.AliasKeyTBS.Extensions
 open ASN1.Spec
 open ASN1.Low
 open X509
-include RIoT.X509.Base
-include RIoT.X509.FWID
-include RIoT.X509.CompositeDeviceID
-include RIoT.X509.Extension
+open RIoT.X509.Base
+open RIoT.X509.FWID
+open RIoT.X509.CompositeDeviceID
+open RIoT.X509.Extension
 open FStar.Integers
 
 module B32 = FStar.Bytes
@@ -14,110 +14,285 @@ module B32 = FStar.Bytes
 open LowParse.Spec.SeqBytes.Base
 open LowParse.Spec.Bytes
 
-(*)
-unfold let elem_t: Type = (t:Type & t)
+#set-options "--z3rlimit 32 --fuel 0 --ifuel 0"
 
-let parser_kind_strong = k: parser_kind {Mkparser_kind'?.parser_kind_subkind k == Some ParserStrong}
+(* Extensions of the AliasKey Certificate
+ * Includes the RIoT Extension (`CompositeDeviceID`) and others
+ * This is the SEQUENCE under the outmost explicit tag
+ * Contains SEQUENCEs of individual extensions ({extID, extValue})
+ * [3] {               <--- The outmost explicit tag
+ *   SEQUENCE {        <--- *HERE*
+ *     SEQUENCE {      <--- Individual extension
+ *       extID   : OID
+ *       extValue: OCTET STRING {..}  <--- Actual extension content enveloped by tag OCTET STRING
+ *     };
+ *     SEQUENCE {..};
+ *     SEQUENCE {..};  <--- Other extensions
+ *   }
+ * }
+ *)
 
-let ser_t: Type
-= ( k: parser_kind_strong &
-    t: Type &
-    p: parser k t &
-    s: serializer p )
-
-let wrap
-  (#k: parser_kind_strong)
-  (#t: Type)
-  (#p: parser k t)
-  (s: serializer p)
-: Tot (ser_t)
-= (|k, t, p, s|)
-
-let ser_list_t: Type = l: list ser_t { 0 < List.length l /\ List.length l <= 5}
-
-let rec sequence_t
-  (l: ser_list_t)
-: Tot (Type)
-  (decreases (List.length l))
-= let l', (|k, t, p, s|) = List.Tot.Base.unsnoc l in
-  List.Tot.Properties.lemma_unsnoc_length l;
-  match l' with
-  | [] -> ( t )
-  | _  -> ( (sequence_t l' `tuple2` t) )
-
-let rec parse_sequence_kind
-  (l: ser_list_t)
-: Tot (parser_kind_strong)
-  (decreases (List.length l))
-= let l', (|k, t, p, s|) = List.Tot.Base.unsnoc l in
-  List.Tot.Properties.lemma_unsnoc_length l;
-  match l' with
-  | [] -> ( k )
-  | _  -> ( (parse_sequence_kind l' `and_then_kind` k) )
-
-let rec parse_sequence
-  (l: ser_list_t)
-: Tot (parser (parse_sequence_kind l) (sequence_t l))
-  (decreases (List.length l))
-= let l', (|k, t, p, s|) = List.Tot.Base.unsnoc l in
-  List.Tot.Properties.lemma_unsnoc_length l;
-  match l' with
-  | [] -> ( p )
-  | _  -> ( (parse_sequence l' `nondep_then` p) )
-
-let rec serialize_sequence
-  (l: ser_list_t)
-: Tot (serializer (parse_sequence l))
-  (decreases (List.length l))
-= let l', (|k, t, p, s|) = List.Tot.Base.unsnoc l in
-  List.Tot.Properties.lemma_unsnoc_length l;
-  match l' with
-  | [] -> ( s )
-  | _  -> ( (serialize_sequence l' `serialize_nondep_then` s) )
-
-(* Test Zone *)
-let l: ser_list_t = [wrap serialize_asn1_integer_TLV;
-                     wrap serialize_asn1_bit_string_TLV]
-
-let msg_t: Type = (t: Type & x: t)
-
-let msg_list_t: Type = l: list msg_t { 0 < List.length l /\ List.length l <= 5}
-
-let wrap_msg
-  (#t: Type)
-  (x: t)
-: Tot (msg_t)
-= (|t, x|)
-
-let rec msg_list_to_tuple_t
-  (l: msg_list_t)
-: Tot (Type)
-  (decreases (List.length l))
-= let l', (|t, x|) = List.Tot.Base.unsnoc l in
-  List.Tot.Properties.lemma_unsnoc_length l;
-  match l' with
-  | [] -> ( t )
-  | _  -> ( msg_list_to_tuple_t l' `tuple2` t )
-
-let rec msg_list_to_tuple
-  (l: msg_list_t)
-: Tot (msg_list_to_tuple_t l)
-  (decreases (List.length l))
-= let l', (|t, x|) = List.Tot.Base.unsnoc l in
-  List.Tot.Properties.lemma_unsnoc_length l;
-  match l' with
-  | [] -> ( x )
-  | _  -> ( (msg_list_to_tuple l', x) )
-
-let x: msg_list_t = [wrap_msg 1ul; wrap_msg ({bs_len = 2ul; bs_unused_bits = 0ul; bs_s = B32.create 1ul 1uy})]
-
-let p = parse_sequence l
-
-let _ assert (get_parser_type p == msg_list_to_tuple_t x)
-
-
-
-type aliasKeyTBS_extensions_t (template_len: asn1_int32) = {
-  aliasKeyTBS_extension_riot: riot_extension_t;
-  aliasKeyTBS_extensions_template: B32.lbytes32 template_len
+(* Exposed message record type (struct) for manipulation *)
+type aliasKeyTBS_extensions_t = {
+  (* More extensions could be added here.
+   * For example:
+   * aliasKeyTBS_extensions_key_usage: key_usage_t;
+   *)
+  aliasKeyTBS_extensions_key_usage: key_usage_t_inbound;
+  aliasKeyTBS_extensions_riot: riot_extension_t_inbound
 }
+
+(* The following helpers should be updated accordingly if
+ * new extensions are added to the type above
+ *)
+(* Actual message tuple type for serialization *)
+let aliasKeyTBS_extensions_t' = (
+  (* More extensions could be added here.
+   * For example:
+   * key_usage_t &
+   *)
+  key_usage_t_inbound `tuple2`
+  riot_extension_t_inbound
+)
+
+(* Conversion of message between record and tuple types *)
+let synth_aliasKeyTBS_extensions_t
+  (x': aliasKeyTBS_extensions_t')
+: GTot (aliasKeyTBS_extensions_t) = {
+  (* More extensions could be added here.
+   * For example:
+   * aliasKeyTBS_extensions_key_usage = fst x;
+   *)
+   aliasKeyTBS_extensions_key_usage = fst x';
+   aliasKeyTBS_extensions_riot      = snd x'
+}
+
+let synth_aliasKeyTBS_extensions_t'
+  (x: aliasKeyTBS_extensions_t)
+: Tot  (x': aliasKeyTBS_extensions_t'
+           {x == synth_aliasKeyTBS_extensions_t x'}) = (
+  (* More extensions could be added here.
+   * For example:
+   * x.aliasKeyTBS_extensions_key_usage,
+   *)
+   x.aliasKeyTBS_extensions_key_usage,
+   x.aliasKeyTBS_extensions_riot
+)
+
+(* Parser Specification for VALUE *)
+let parse_aliasKeyTBS_extensions
+: parser _ (aliasKeyTBS_extensions_t)
+= parse_x509_key_usage
+  `nondep_then`
+  parse_riot_extension_sequence_TLV
+  `parse_synth`
+  synth_aliasKeyTBS_extensions_t
+
+(* Serializer Specification for VALUE *)
+let serialize_aliasKeyTBS_extensions
+: serializer (parse_aliasKeyTBS_extensions)
+= serialize_synth
+  (* p1 *) (parse_x509_key_usage
+            `nondep_then`
+            parse_riot_extension_sequence_TLV)
+  (* f2 *) (synth_aliasKeyTBS_extensions_t)
+  (* s1 *) (serialize_x509_key_usage
+            `serialize_nondep_then`
+            serialize_riot_extension_sequence_TLV)
+  (* g1 *) (synth_aliasKeyTBS_extensions_t')
+  (* prf*) ()
+
+(* Lemmas for serialization *)
+let lemma_serialize_aliasKeyTBS_extensions_unfold
+  (x: aliasKeyTBS_extensions_t)
+: Lemma (
+  serialize_aliasKeyTBS_extensions `serialize` x ==
+  (serialize_x509_key_usage `serialize` x.aliasKeyTBS_extensions_key_usage)
+  `Seq.append`
+  (serialize_riot_extension_sequence_TLV `serialize` x.aliasKeyTBS_extensions_riot)
+)
+= serialize_nondep_then_eq
+  (* s1 *) (serialize_x509_key_usage)
+  (* s2 *) (serialize_riot_extension_sequence_TLV)
+  (* in *) (synth_aliasKeyTBS_extensions_t' x);
+  serialize_synth_eq
+  (* p1 *) (parse_x509_key_usage
+            `nondep_then`
+            parse_riot_extension_sequence_TLV)
+  (* f2 *) (synth_aliasKeyTBS_extensions_t)
+  (* s1 *) (serialize_x509_key_usage
+            `serialize_nondep_then`
+            serialize_riot_extension_sequence_TLV)
+  (* g1 *) (synth_aliasKeyTBS_extensions_t')
+  (* prf*) ()
+  (* in *) (x)
+
+let length_of_aliasKeyTBS_extensions_payload
+    (ku: key_usage_t)
+    (version: datatype_of_asn1_type INTEGER)
+= length_of_riot_extension version +
+  length_of_x509_key_usage ku
+
+let len_of_aliasKeyTBS_extensions_payload
+    (ku: key_usage_t)
+    (version: datatype_of_asn1_type INTEGER
+              { length_of_aliasKeyTBS_extensions_payload ku version
+                <= asn1_value_length_max_of_type SEQUENCE })
+: Tot (len: asn1_TLV_int32_of_type SEQUENCE
+            { v len == length_of_aliasKeyTBS_extensions_payload ku version })
+= len_of_riot_extension version +
+  len_of_x509_key_usage ku
+
+#push-options "--query_stats --z3rlimit 64 --fuel 0 --ifuel 0"
+let lemma_serialize_aliasKeyTBS_extensions_size
+  (x: aliasKeyTBS_extensions_t)
+: Lemma (
+  (* unfold *)
+  length_of_opaque_serialization (serialize_aliasKeyTBS_extensions)      x ==
+  length_of_opaque_serialization (serialize_riot_extension_sequence_TLV) x.aliasKeyTBS_extensions_riot +
+  length_of_opaque_serialization (serialize_x509_key_usage)              x.aliasKeyTBS_extensions_key_usage /\
+  (* exact size of the VALUE of SEQUENCE
+   * For now its just the size of the RIoT Extension
+   *)
+  length_of_opaque_serialization (serialize_aliasKeyTBS_extensions)      x
+  == length_of_aliasKeyTBS_extensions_payload
+       (snd x.aliasKeyTBS_extensions_key_usage)
+       (x.aliasKeyTBS_extensions_riot.x509_extValue_riot.riot_version)
+  (* upper bound *)
+  // length_of_opaque_serialization (serialize_aliasKeyTBS_extensions)      x
+  // <= 117
+)
+= lemma_serialize_aliasKeyTBS_extensions_unfold x;
+    lemma_serialize_riot_extension_sequence_TLV_size_exact x.aliasKeyTBS_extensions_riot;
+    lemma_serialize_x509_key_usage_size_exact x.aliasKeyTBS_extensions_key_usage
+#pop-options
+
+(*
+ * SEQUENCE serializer
+ *)
+(* aliasKeyTBS_extensions: inbound sub type for SEQUENCE TLV*)
+// unfold
+let aliasKeyTBS_extensions_t_inbound
+= inbound_sequence_value_of (serialize_aliasKeyTBS_extensions)
+
+(* aliasKeyTBS_extensions: parser for TLV *)
+let parse_aliasKeyTBS_extensions_sequence_TLV
+: parser (parse_asn1_envelop_tag_with_TLV_kind SEQUENCE) (aliasKeyTBS_extensions_t_inbound)
+= aliasKeyTBS_extensions_t_inbound
+  `coerce_parser`
+  parse_asn1_sequence_TLV (serialize_aliasKeyTBS_extensions)
+
+(* aliasKeyTBS_extensions: serializer for TLV *)
+let serialize_aliasKeyTBS_extensions_sequence_TLV
+: serializer (parse_aliasKeyTBS_extensions_sequence_TLV)
+= coerce_parser_serializer
+  (* t *) (parse_aliasKeyTBS_extensions_sequence_TLV)
+  (* s *) (serialize_asn1_sequence_TLV (serialize_aliasKeyTBS_extensions))
+  (*prf*) ()
+
+(* aliasKeyTBS_extensions: lemmas for TLV *)
+let lemma_serialize_aliasKeyTBS_extensions_sequence_TLV_unfold
+  (x: aliasKeyTBS_extensions_t_inbound)
+: Lemma ( predicate_serialize_asn1_sequence_TLV_unfold serialize_aliasKeyTBS_extensions x )
+= lemma_serialize_asn1_sequence_TLV_unfold serialize_aliasKeyTBS_extensions x
+
+let lemma_serialize_aliasKeyTBS_extensions_sequence_TLV_size
+  (x: aliasKeyTBS_extensions_t_inbound)
+: Lemma ( predicate_serialize_asn1_sequence_TLV_size serialize_aliasKeyTBS_extensions x )
+= lemma_serialize_asn1_sequence_TLV_size serialize_aliasKeyTBS_extensions x
+
+let length_of_aliasKeyTBS_extensions
+    (ku: key_usage_t)
+    (version: datatype_of_asn1_type INTEGER)
+: GTot (asn1_TLV_length_of_type SEQUENCE)
+= length_of_TLV SEQUENCE
+    (length_of_riot_extension version +
+     length_of_x509_key_usage ku)
+
+#push-options "--z3rlimit 64 --fuel 0 --ifuel 0"
+let len_of_aliasKeyTBS_extensions
+    (ku: key_usage_t)
+    (version: datatype_of_asn1_type INTEGER
+              { length_of_aliasKeyTBS_extensions ku version
+                <= asn1_value_length_max_of_type SEQUENCE })
+: Tot (len: asn1_TLV_int32_of_type SEQUENCE
+            { v len == length_of_aliasKeyTBS_extensions ku version })
+= len_of_TLV SEQUENCE
+    (len_of_riot_extension version +
+     len_of_x509_key_usage ku)
+#pop-options
+
+#push-options "--z3rlimit 64 --fuel 0 --ifuel 0"
+let lemma_serialize_aliasKeyTBS_extensions_sequence_TLV_size_exact
+  (x: aliasKeyTBS_extensions_t_inbound)
+: Lemma (
+  (* exact size of the VALUE of SEQUENCE
+   * For now its just the size of the RIoT Extension
+   *)
+  length_of_opaque_serialization (serialize_aliasKeyTBS_extensions_sequence_TLV) x
+  == length_of_aliasKeyTBS_extensions
+       (snd x.aliasKeyTBS_extensions_key_usage)
+       (x.aliasKeyTBS_extensions_riot.x509_extValue_riot.riot_version)
+  (* upper bound *)
+  // length_of_opaque_serialization (serialize_aliasKeyTBS_extensions_sequence_TLV)      x
+  // <= 6 +
+  //      117
+)
+= lemma_serialize_aliasKeyTBS_extensions_sequence_TLV_size x;
+  lemma_serialize_aliasKeyTBS_extensions_size x
+#pop-options
+
+(*
+ * Low Level Serializer
+ *)
+(* aliasKeyTBS_extensions: low level serializer for VALUE *)
+let serialize32_aliasKeyTBS_extensions_backwards
+: serializer32_backwards (serialize_aliasKeyTBS_extensions)
+= serialize32_synth_backwards
+  (* s32 *) (serialize32_x509_key_usage_backwards
+             `serialize32_nondep_then_backwards`
+             serialize32_riot_extension_sequence_TLV_backwards)
+  (* f2  *) synth_aliasKeyTBS_extensions_t
+  (* g1  *) synth_aliasKeyTBS_extensions_t'
+  (* g1' *) synth_aliasKeyTBS_extensions_t'
+  (* prf *) ()
+
+(* aliasKeyTBS_extensions: low level serializer for SEQUENCE TLV *)
+let serialize32_aliasKeyTBS_extensions_sequence_TLV_backwards
+: serializer32_backwards (serialize_aliasKeyTBS_extensions_sequence_TLV)
+= coerce_serializer32_backwards
+  (* s2  *) (serialize_aliasKeyTBS_extensions_sequence_TLV)
+  (* s32 *) (serialize32_asn1_sequence_TLV_backwards
+             (* ls *) (serialize32_aliasKeyTBS_extensions_backwards))
+  (* prf *) ()
+
+#push-options "--z3rlimit 64 --fuel 0 --ifuel 0"
+let x509_get_aliasKeyTBS_extensions
+  (ku: key_usage_t)
+  (version: datatype_of_asn1_type INTEGER
+            { length_of_aliasKeyTBS_extensions ku version
+              <= asn1_value_length_max_of_type SEQUENCE })
+  (fwid: B32.lbytes32 32ul)
+  (deviceIDPub: B32.lbytes32 32ul)
+: Tot (aliasKeyTBS_extensions_t_inbound)
+=
+  let riot_extension= x509_get_riot_extension
+                        version
+                        fwid
+                        deviceIDPub in
+  (* Prf *) lemma_serialize_riot_extension_sequence_TLV_size_exact riot_extension;
+
+  let key_usage = x509_get_key_usage ku in
+  (* Prf *) lemma_serialize_x509_key_usage_size_exact key_usage;
+
+  let aliasKeyTBS_extensions: aliasKeyTBS_extensions_t = {
+    aliasKeyTBS_extensions_riot = riot_extension;
+    aliasKeyTBS_extensions_key_usage = key_usage
+  } in
+  (* Prf *) lemma_serialize_aliasKeyTBS_extensions_unfold aliasKeyTBS_extensions;
+  (* Prf *) lemma_serialize_aliasKeyTBS_extensions_size   aliasKeyTBS_extensions;
+  (* Prf *) assert ( length_of_opaque_serialization serialize_aliasKeyTBS_extensions aliasKeyTBS_extensions
+                     <= asn1_value_length_max_of_type SEQUENCE );
+
+(*return*) aliasKeyTBS_extensions
+#pop-options
