src/riot/x509/X509.ExtFields.KeyUsage.fst
@@ -5,6 +5,7 @@ open LowParse.Spec.Combinators
 
 open ASN1.Base
 open ASN1.Spec
+open ASN1.Low
 
 open X509.Base
 
@@ -13,24 +14,29 @@ module B32 = FStar.Bytes
 open FStar.Integers
 
 (*
-/*
- * X.509 v3 Key Usage Extension flags
- * Reminder: update x509_info_key_usage() when adding new flags.
- */
-#define MBEDTLS_X509_KU_DIGITAL_SIGNATURE            (0x80)  /* bit 0 */
-#define MBEDTLS_X509_KU_NON_REPUDIATION              (0x40)  /* bit 1 */
-#define MBEDTLS_X509_KU_KEY_ENCIPHERMENT             (0x20)  /* bit 2 */
-#define MBEDTLS_X509_KU_DATA_ENCIPHERMENT            (0x10)  /* bit 3 */
-#define MBEDTLS_X509_KU_KEY_AGREEMENT                (0x08)  /* bit 4 */
-#define MBEDTLS_X509_KU_KEY_CERT_SIGN                (0x04)  /* bit 5 */
-#define MBEDTLS_X509_KU_CRL_SIGN                     (0x02)  /* bit 6 */
-#define MBEDTLS_X509_KU_ENCIPHER_ONLY                (0x01)  /* bit 7 */
-#define MBEDTLS_X509_KU_DECIPHER_ONLY              (0x8000)  /* bit 8 */
-*)
-(*)
-let key_usage_t = i: datatype_of_asn1_type INTEGER
-                     { 0l < i /\ (* at least one usage *)
-                      (i <= 0xFFl \/ i / 0x100l == 0x80l) }
+ * /*
+ *  * X.509 v3 Key Usage Extension flags
+ *  * Reminder: update x509_info_key_usage() when adding new flags.
+ *  */
+ * #define MBEDTLS_X509_KU_DIGITAL_SIGNATURE            (0x80)  /* bit 0 */
+ * #define MBEDTLS_X509_KU_NON_REPUDIATION              (0x40)  /* bit 1 */
+ * #define MBEDTLS_X509_KU_KEY_ENCIPHERMENT             (0x20)  /* bit 2 */
+ * #define MBEDTLS_X509_KU_DATA_ENCIPHERMENT            (0x10)  /* bit 3 */
+ * #define MBEDTLS_X509_KU_KEY_AGREEMENT                (0x08)  /* bit 4 */
+ * #define MBEDTLS_X509_KU_KEY_CERT_SIGN                (0x04)  /* bit 5 */
+ * #define MBEDTLS_X509_KU_CRL_SIGN                     (0x02)  /* bit 6 */
+ * #define MBEDTLS_X509_KU_ENCIPHER_ONLY                (0x01)  /* bit 7 */
+ * #define MBEDTLS_X509_KU_DECIPHER_ONLY              (0x8000)  /* bit 8 */
+ *)
+
+let valid_key_usage
+  (i: int_32)
+: Type0
+= 0l < i /\ (* at least one usage *)
+  (i <= 0xFFl \/ i / 0x100l == 0x80l)
+
+let key_usage_t = i: int_32
+                     { valid_key_usage i }
 
 let x509_KU_DIGITAL_SIGNATURE :key_usage_t = 0x80l    (* bit 0 *)
 let x509_KU_NON_REPUDIATION   :key_usage_t = 0x40l    (* bit 1 *)
@@ -42,42 +48,58 @@ let x509_KU_CRL_SIGN          :key_usage_t = 0x02l    (* bit 6 *)
 let x509_KU_ENCIPHER_ONLY     :key_usage_t = 0x01l    (* bit 7 *)
 let x509_KU_DECIPHER_ONLY     :key_usage_t = 0x8000l  (* bit 8 *)
 
-let filter_x509_key_usage
+(* FIXME: Can we normalize bitwise operators? *)
+let lemma_key_usage_close_under_or
+  (ku1 ku2: key_usage_t)
+: Lemma (
+  valid_key_usage (ku1 |^ ku2)
+)
+= admit()
+
+let op_ku_with
+  (ku1 ku2: key_usage_t)
+: Tot (ku: key_usage_t
+           { ku == (ku1 |^ ku2) })
+= [@inline_let]let ku: int_32 = ku1 |^ ku2 in
+  lemma_key_usage_close_under_or ku1 ku2;
+  ku
+
+let _filter_x509_key_usage_payload
   (bs: datatype_of_asn1_type BIT_STRING)
 : GTot bool
 = bs.bs_len = 3ul &&
   bs.bs_unused_bits = 7ul &&
   (* NOTE: RFC 5280 4.2.1.3:
-//            When the keyUsage extension appears in a certificate,
-//            at least one of the bits MUST be set to 1.*)
+   *       When the keyUsage extension appears in a certificate,
+   *       at least one of the bits MUST be set to 1. *)
   (B32.index bs.bs_s 1 = 0x80uy ||
    B32.index bs.bs_s 1 = 0x00uy && B32.index bs.bs_s 0 > 0x00uy)
 
-let synth_x509_key_usage
-  (bs: parse_filter_refine filter_x509_key_usage)
+let _synth_x509_key_usage_payload
+  (bs: parse_filter_refine _filter_x509_key_usage_payload)
 : GTot (key_usage_t)
 = cast #(Unsigned W8) #(Signed W32) (B32.index bs.bs_s 0) +
   ((cast #(Unsigned W8) #(Signed W32) (B32.index bs.bs_s 1)) * 0x100l)
 
-let lemma_synth_x509_key_usage_injective'
-  (bs1 bs2: parse_filter_refine filter_x509_key_usage)
+let lemma_synth_x509_key_usage_payload_injective'
+  (bs1 bs2: parse_filter_refine _filter_x509_key_usage_payload)
 : Lemma
-  (requires synth_x509_key_usage bs1 == synth_x509_key_usage bs2)
+  (requires _synth_x509_key_usage_payload bs1 == _synth_x509_key_usage_payload bs2)
   (ensures bs1 == bs2)
 = admit ()
 
 let lemma_synth_x509_key_usage_injective ()
 : Lemma (
-  synth_injective synth_x509_key_usage
+  synth_injective _synth_x509_key_usage_payload
 )
 = synth_injective_intro'
-  (* f *) synth_x509_key_usage
-  (*prf*) lemma_synth_x509_key_usage_injective'
+  (* f *) _synth_x509_key_usage_payload
+  (*prf*) lemma_synth_x509_key_usage_payload_injective'
 
-let synth_x509_key_usage_inverse
+let _synth_x509_key_usage_payload_inverse
   (ku: key_usage_t)
-: GTot (bs: parse_filter_refine filter_x509_key_usage
-            { synth_x509_key_usage bs == ku })
+: GTot (bs: parse_filter_refine _filter_x509_key_usage_payload
+            { _synth_x509_key_usage_payload bs == ku })
 = let b0: byte = cast (ku % 0x100l) in
   let b1: byte = cast (ku / 0x100l) in
   let s = Seq.createL [b0; b1] in
@@ -86,120 +108,244 @@ let synth_x509_key_usage_inverse
     bs_unused_bits = 7ul;
     bs_s           = s32 }
 
-let parse_x509_key_usage
+let _parse_x509_key_usage_payload
 : parser _ key_usage_t
 = lemma_synth_x509_key_usage_injective ();
   parse_asn1_TLV_of_type BIT_STRING
   `parse_filter`
-  filter_x509_key_usage
+  _filter_x509_key_usage_payload
   `parse_synth`
-  synth_x509_key_usage
+  _synth_x509_key_usage_payload
 
-let serialize_x509_key_usage
-: serializer parse_x509_key_usage
+let _serialize_x509_key_usage_payload
+: serializer _parse_x509_key_usage_payload
 = serialize_synth
   (* p1 *) (parse_asn1_TLV_of_type BIT_STRING
             `parse_filter`
-            filter_x509_key_usage)
-  (* f2 *) (synth_x509_key_usage)
+            _filter_x509_key_usage_payload)
+  (* f2 *) (_synth_x509_key_usage_payload)
   (* s1 *) (serialize_asn1_TLV_of_type BIT_STRING
             `serialize_filter`
-            filter_x509_key_usage)
-  (* g1 *) (synth_x509_key_usage_inverse)
+            _filter_x509_key_usage_payload)
+  (* g1 *) (_synth_x509_key_usage_payload_inverse)
   (* Prf*) (lemma_synth_x509_key_usage_injective ())
 
-let lemma_serialize_x509_key_usage_unfold
+let lemma_serialize_x509_key_usage_payload_unfold
   (ku: key_usage_t)
 : Lemma (
-  serialize serialize_x509_key_usage ku ==
-  serialize (serialize_asn1_TLV_of_type BIT_STRING) (synth_x509_key_usage_inverse ku)
+  serialize _serialize_x509_key_usage_payload ku ==
+  serialize (serialize_asn1_TLV_of_type BIT_STRING) (_synth_x509_key_usage_payload_inverse ku)
 )
 = serialize_synth_eq
   (* p1 *) (parse_asn1_TLV_of_type BIT_STRING
             `parse_filter`
-            filter_x509_key_usage)
-  (* f2 *) (synth_x509_key_usage)
+            _filter_x509_key_usage_payload)
+  (* f2 *) (_synth_x509_key_usage_payload)
   (* s1 *) (serialize_asn1_TLV_of_type BIT_STRING
             `serialize_filter`
-            filter_x509_key_usage)
-  (* g1 *) (synth_x509_key_usage_inverse)
+            _filter_x509_key_usage_payload)
+  (* g1 *) (_synth_x509_key_usage_payload_inverse)
   (* Prf*) (lemma_synth_x509_key_usage_injective ())
   (* in *) (ku)
 
-let lemma_serialize_x509_key_usage_size
+let lemma_serialize_x509_key_usage_payload_size
   (ku: key_usage_t)
 : Lemma (
-  Seq.length (serialize serialize_x509_key_usage ku) ==
-  length_of_asn1_primitive_TLV #BIT_STRING (synth_x509_key_usage_inverse ku)
+  length_of_opaque_serialization _serialize_x509_key_usage_payload ku ==
+  length_of_asn1_primitive_TLV #BIT_STRING (_synth_x509_key_usage_payload_inverse ku)
 )
-= lemma_serialize_x509_key_usage_unfold ku
+= lemma_serialize_x509_key_usage_payload_unfold ku
 
-// let parse_envelop_OID_with
-//   (oid: datatype_of_asn1_type OID)
-//   (#k: parser_kind)
-//   (#t: Type0)
-//   (#p: parser k t)
-//   (s: serializer p)
-// : parser _ _
-// = parse_asn1_oid_TLV
-//   `parse_filter`
-//   (fun x -> x = oid)
-//   `nondep_then`
-//   p
+(* Complete X509 Key Usage Parser and Serializer for
+ *
+ *  SEQUENCE {
+ *    extID   : OID
+ *    extValue: OCTET_STRING {
+ *      key_usage    : key_usage_t
+ *    }
+ *  }
+ *
+ *)
 
-let parse_x509_key_usage_sequence_TLV
-= parse_asn1_sequence_TLV
+let key_usage_t_inbound
+= inbound_sequence_value_of
     (OID_KEY_USAGE
      `serialize_envelop_OID_with`
-     serialize_x509_key_usage)
+    (OCTET_STRING
+     `serialize_asn1_envelop_tag_with_TLV`
+     _serialize_x509_key_usage_payload))
 
-let serialize_x509_key_usage_sequence_TLV
-= serialize_asn1_sequence_TLV
+let parse_x509_key_usage
+: parser (parse_asn1_envelop_tag_with_TLV_kind SEQUENCE) key_usage_t_inbound
+= key_usage_t_inbound
+  `coerce_parser`
+ (parse_asn1_sequence_TLV
     (OID_KEY_USAGE
      `serialize_envelop_OID_with`
-     serialize_x509_key_usage)
+    (OCTET_STRING
+     `serialize_asn1_envelop_tag_with_TLV`
+     _serialize_x509_key_usage_payload)))
 
-let lemma_serialize_x509_key_usage_sequence_TLV_unfold
+let serialize_x509_key_usage
+: serializer (parse_x509_key_usage)
+= coerce_parser_serializer
+  (* p *) (parse_x509_key_usage)
+  (* s *) (serialize_asn1_sequence_TLV
+            (OID_KEY_USAGE
+             `serialize_envelop_OID_with`
+            (OCTET_STRING
+             `serialize_asn1_envelop_tag_with_TLV`
+             _serialize_x509_key_usage_payload)))
+  (*prf*) ()
+
+let lemma_serialize_x509_key_usage_unfold
+  (x: key_usage_t_inbound)
+: Lemma ( predicate_serialize_asn1_sequence_TLV_unfold
+            (OID_KEY_USAGE
+             `serialize_envelop_OID_with`
+            (OCTET_STRING
+             `serialize_asn1_envelop_tag_with_TLV`
+             _serialize_x509_key_usage_payload))
+            x )
 = lemma_serialize_asn1_sequence_TLV_unfold
     (OID_KEY_USAGE
      `serialize_envelop_OID_with`
-     serialize_x509_key_usage)
+    (OCTET_STRING
+             `serialize_asn1_envelop_tag_with_TLV`
+             _serialize_x509_key_usage_payload))
+    x
 
-let lemma_serialize_x509_key_usage_sequence_TLV_size
+let lemma_serialize_x509_key_usage_size
+  (x: key_usage_t_inbound)
+: Lemma ( predicate_serialize_asn1_sequence_TLV_size
+            (OID_KEY_USAGE
+             `serialize_envelop_OID_with`
+            (OCTET_STRING
+             `serialize_asn1_envelop_tag_with_TLV`
+             _serialize_x509_key_usage_payload))
+            x )
 = lemma_serialize_asn1_sequence_TLV_size
     (OID_KEY_USAGE
      `serialize_envelop_OID_with`
-     serialize_x509_key_usage)
+    (OCTET_STRING
+             `serialize_asn1_envelop_tag_with_TLV`
+             _serialize_x509_key_usage_payload))
+    x
+
+let length_of_x509_key_usage
+  (ku: key_usage_t)
+: GTot (asn1_TLV_length_of_type SEQUENCE)
+= length_of_TLV
+    SEQUENCE
+    ( length_of_asn1_primitive_TLV #BIT_STRING (_synth_x509_key_usage_payload_inverse ku) +
+      ( length_of_TLV
+          OCTET_STRING
+          ( length_of_asn1_primitive_TLV #OID OID_KEY_USAGE ) ) )
+
+#restart-solver
+#push-options "--z3rlimit 64 --fuel 0 --fuel 0"
+let lemma_serialize_x509_key_usage_size_exact
+  (x: key_usage_t_inbound)
+: Lemma (
+  length_of_opaque_serialization serialize_x509_key_usage x
+  == length_of_x509_key_usage (snd x)
+)
+= lemma_serialize_x509_key_usage_size x;
+  (**) lemma_serialize_envelop_OID_with_size
+         (fst x)
+         (OCTET_STRING
+          `serialize_asn1_envelop_tag_with_TLV`
+          _serialize_x509_key_usage_payload)
+         x;
+       (**) lemma_serialize_asn1_oid_TLV_of_size (fst x) (fst x);
+       (**) lemma_serialize_asn1_envelop_tag_with_TLV_size
+              (OCTET_STRING)
+              (_serialize_x509_key_usage_payload)
+              (snd x);
+            (**) lemma_serialize_x509_key_usage_payload_size (snd x)
+#pop-options
 
 open ASN1.Low
 
-let synth_x509_key_usage_inverse_impl
+#push-options "--z3rlimit 32"
+let _synth_x509_key_usage_payload_inverse_impl
   (ku: key_usage_t)
-: Tot (bs: parse_filter_refine filter_x509_key_usage
-           { bs == synth_x509_key_usage_inverse ku })
-= let b0: byte = cast (ku % 0x100l) in
-  let b1: byte = cast (ku / 0x100l) in
+: Tot (bs: parse_filter_refine _filter_x509_key_usage_payload
+           { bs == _synth_x509_key_usage_payload_inverse ku })
+= let b0: byte = FStar.Int.Cast.int32_to_uint8 (ku % 0x100l) in
+  let b1: byte = FStar.Int.Cast.int32_to_uint8 (ku / 0x100l) in
   let s32 = B32.(create 1ul b0 `append` create 1ul b1) in
   (* Prf *) B32.extensionality s32 (B32.hide (Seq.createL [b0; b1]));
   { bs_len         = 3ul;
     bs_unused_bits = 7ul;
     bs_s           = s32 }
+#pop-options
 
-let serialize32_x509_key_usage_backwards
-: serializer32_backwards (serialize_x509_key_usage)
+#push-options "--z3rlimit 32 --fuel 0 --fuel 0"
+let len_of_x509_key_usage
+  (ku: key_usage_t)
+: Tot (len: asn1_TLV_int32_of_type SEQUENCE
+            { v len == length_of_x509_key_usage ku })
+= len_of_TLV
+    SEQUENCE
+    ( len_of_asn1_primitive_TLV #BIT_STRING (_synth_x509_key_usage_payload_inverse_impl ku) +
+      ( len_of_TLV
+          OCTET_STRING
+          ( len_of_asn1_primitive_TLV #OID OID_KEY_USAGE ) ) )
+#pop-options
+
+let _serialize32_x509_key_usage_payload_backwards
+: serializer32_backwards (_serialize_x509_key_usage_payload)
 = serialize32_synth_backwards
   (* s1 *) (serialize32_asn1_TLV_backwards_of_type BIT_STRING
             `serialize32_filter_backwards`
-            filter_x509_key_usage)
-  (* f2 *) (synth_x509_key_usage)
-  (* g1 *) (synth_x509_key_usage_inverse)
-  (* g1'*) (synth_x509_key_usage_inverse_impl)
+            _filter_x509_key_usage_payload)
+  (* f2 *) (_synth_x509_key_usage_payload)
+  (* g1 *) (_synth_x509_key_usage_payload_inverse)
+  (* g1'*) (_synth_x509_key_usage_payload_inverse_impl)
   (* prf*) (lemma_synth_x509_key_usage_injective ())
 
-let serialize32_x509_key_usage_sequence_TLV_backwards
-: serializer32_backwards (serialize_x509_key_usage_sequence_TLV)
+let serialize32_x509_key_usage_backwards
+: serializer32_backwards (serialize_x509_key_usage)
 = lemma_synth_x509_key_usage_injective ();
-  serialize32_asn1_sequence_TLV_backwards
-    (OID_KEY_USAGE
-     `serialize32_envelop_OID_with_backwards`
-     serialize32_x509_key_usage_backwards)
+  coerce_serializer32_backwards
+  (* s2  *) (serialize_x509_key_usage)
+  (* s32 *) (serialize32_asn1_sequence_TLV_backwards
+              (OID_KEY_USAGE
+               `serialize32_envelop_OID_with_backwards`
+              (OCTET_STRING
+               `serialize32_asn1_envelop_tag_with_TLV_backwards`
+               _serialize32_x509_key_usage_payload_backwards)))
+  (* prf *) ()
+
+///
+///
+/// Helper constructor
+#push-options "--z3rlimit 32 --fuel 0 --fuel 0"
+let x509_get_key_usage
+  (ku: key_usage_t)
+// : Tot (key_usage_t_inbound)
+=
+  (* Prf *) lemma_serialize_x509_key_usage_payload_size ku;
+  let x: OID_KEY_USAGE
+         `envelop_OID_with_t`
+        (OCTET_STRING
+         `inbound_envelop_tag_with_value_of`
+         _serialize_x509_key_usage_payload)
+    = ( OID_KEY_USAGE, ku ) in
+
+  (* Prf *) lemma_serialize_envelop_OID_with_size
+              (fst x)
+              (OCTET_STRING
+               `serialize_asn1_envelop_tag_with_TLV`
+               _serialize_x509_key_usage_payload)
+              (x);
+  (* Prf *) (**) lemma_serialize_asn1_oid_TLV_of_size (fst x) (fst x);
+  (* Prf *) (**) lemma_serialize_asn1_envelop_tag_with_TLV_size
+                   (OCTET_STRING)
+                   (_serialize_x509_key_usage_payload)
+                   (snd x);
+  (* Prf *)      (**) lemma_serialize_x509_key_usage_payload_size (snd x);
+
+(*return*) x <: key_usage_t_inbound
+#pop-options
