src/riot/RIoT.X509.Base.fst
@@ -1,5 +1,16 @@
 module RIoT.X509.Base
 open X509.Base
+open X509.ExtFields.KeyUsage
+
+let aliasKeyCrt_key_usage: key_usage_t
+= x509_KU_KEY_CERT_SIGN
+  (*
+   * Adding more key usage bits for test only. According to the
+   * [reference implementation](https://github.com/microsoft/RIoT/blob/master/Reference/RIoT/RIoTCrypt/include/x509bldr.h#L22),
+   * Only the KeyCertSign bit is set.
+   *)
+  `op_ku_with` x509_KU_DIGITAL_SIGNATURE
+  `op_ku_with` x509_KU_CRL_SIGN
 
 // inline_for_extraction
 // let alg_DeviceID = AlgID_Ed25519
