src/riot/x509/X509.BasicFields.Extensions.fst
@@ -1,0 +1,231 @@
+module X509.BasicFields.Extensions
+
+open LowParse.Spec.Base
+open LowParse.Spec.Combinators
+
+open ASN1.Base
+open ASN1.Spec
+open ASN1.Low
+
+open X509.Base
+open FStar.Integers
+
+module B32 = FStar.Bytes
+
+let x509_extensions_outmost_explicit_tag: asn1_tag_t
+= CUSTOM_TAG CONTEXT_SPECIFIC CONSTRUCTED 3uy
+
+inline_for_extraction
+let x509_extensions_t_inbound
+  (#k: parser_kind)
+  (#t: Type0)
+  (#p: parser k t)
+  (s: serializer p)
+= inbound_envelop_tag_with_value_of
+  (* tag *) x509_extensions_outmost_explicit_tag
+  (*  s  *) s
+
+let parse_x509_extensions_TLV
+  (#k: parser_kind)
+  (#t: Type0)
+  (#p: parser k t)
+  (s: serializer p)
+: parser (parse_asn1_envelop_tag_with_TLV_kind x509_extensions_outmost_explicit_tag) (x509_extensions_t_inbound s)
+= x509_extensions_t_inbound s
+  `coerce_parser`
+  parse_asn1_envelop_tag_with_TLV
+  (* tag *) x509_extensions_outmost_explicit_tag
+  (*  s  *) s
+
+let serialize_x509_extensions_TLV
+  (#k: parser_kind)
+  (#t: Type0)
+  (#p: parser k t)
+  (s: serializer p)
+: serializer (parse_x509_extensions_TLV s)
+= coerce_parser_serializer
+  (* p *) (parse_x509_extensions_TLV s)
+  (* s *) (serialize_asn1_envelop_tag_with_TLV
+           (* tag *) x509_extensions_outmost_explicit_tag
+           (*  s  *) s)
+  (*prf*) ()
+
+let lemma_serialize_x509_extensions_TLV_unfold
+  (#k: parser_kind)
+  (#t: Type0)
+  (#p: parser k t)
+  (s: serializer p)
+  (x: x509_extensions_t_inbound s)
+: Lemma ( predicate_serialize_asn1_envelop_tag_with_TLV_unfold x509_extensions_outmost_explicit_tag s x )
+= lemma_serialize_asn1_envelop_tag_with_TLV_unfold x509_extensions_outmost_explicit_tag s x
+
+let lemma_serialize_x509_extensions_TLV_size
+  (#k: parser_kind)
+  (#t: Type0)
+  (#p: parser k t)
+  (s: serializer p)
+  (x: x509_extensions_t_inbound s)
+: Lemma ( predicate_serialize_asn1_envelop_tag_with_TLV_size x509_extensions_outmost_explicit_tag s x )
+= lemma_serialize_asn1_envelop_tag_with_TLV_size x509_extensions_outmost_explicit_tag s x
+
+let length_of_x509_extensions
+  (l: asn1_value_length_of_type x509_extensions_outmost_explicit_tag)
+: GTot (asn1_TLV_length_of_type x509_extensions_outmost_explicit_tag)
+= length_of_TLV x509_extensions_outmost_explicit_tag l
+
+let len_of_x509_extensions
+  (len_payload: asn1_value_int32_of_type x509_extensions_outmost_explicit_tag)
+: Tot (len: asn1_TLV_int32_of_type x509_extensions_outmost_explicit_tag
+            { v len == length_of_x509_extensions (v len_payload) })
+= len_of_TLV x509_extensions_outmost_explicit_tag len_payload
+
+inline_for_extraction
+let serialize32_x509_extensions_TLV_backwards
+  (#k: parser_kind)
+  (#t: Type0)
+  (#p: parser k t)
+  (#s: serializer p)
+  (s32: serializer32_backwards s)
+: serializer32_backwards (serialize_x509_extensions_TLV s)
+= coerce_serializer32_backwards
+  (* s2  *) (serialize_x509_extensions_TLV s)
+  (* s32 *) (serialize32_asn1_envelop_tag_with_TLV_backwards
+             (* tag *) x509_extensions_outmost_explicit_tag
+             (* s32 *) s32)
+  (* prf *) ()
+
+
+(*)
+(* inner sequence *)
+
+let x509_extensions_inner_sequence_t_inbound
+  (#k: parser_kind)
+  (#t: Type0)
+  (#p: parser k t)
+  (s: serializer p)
+= inbound_sequence_value_of s
+
+let parse_x509_extensions_inner_sequence_TLV
+  (#k: parser_kind)
+  (#t: Type0)
+  (#p: parser k t)
+  (s: serializer p)
+: parser (parse_asn1_envelop_tag_with_TLV_kind SEQUENCE) (x509_extensions_inner_sequence_t_inbound s)
+= x509_extensions_inner_sequence_t_inbound s
+  `coerce_parser`
+  parse_asn1_sequence_TLV s
+
+let serialize_x509_extensions_inner_sequence_TLV
+  (#k: parser_kind)
+  (#t: Type0)
+  (#p: parser k t)
+  (s: serializer p)
+: serializer (parse_x509_extensions_inner_sequence_TLV s)
+= coerce_parser_serializer
+  (* t *) (parse_x509_extensions_inner_sequence_TLV s)
+  (* s *) (serialize_asn1_sequence_TLV s)
+  (*prf*) ()
+
+let lemma_serialize_x509_extensions_inner_sequence_TLV_unfold
+  (#k: parser_kind)
+  (#t: Type0)
+  (#p: parser k t)
+  (s: serializer p)
+  (x: x509_extensions_inner_sequence_t_inbound s)
+: Lemma ( predicate_serialize_asn1_sequence_TLV_unfold s x )
+= lemma_serialize_asn1_sequence_TLV_unfold s x
+
+let lemma_serialize_x509_extensions_inner_sequence_TLV_size
+  (#k: parser_kind)
+  (#t: Type0)
+  (#p: parser k t)
+  (s: serializer p)
+  (x: x509_extensions_inner_sequence_t_inbound s)
+: Lemma ( predicate_serialize_asn1_sequence_TLV_size s x )
+= lemma_serialize_asn1_sequence_TLV_size s x
+
+let serialize32_x509_extensions_inner_sequence_TLV_backwards
+  (#k: parser_kind)
+  (#t: Type0)
+  (#p: parser k t)
+  (#s: serializer p)
+  (s32: serializer32_backwards s)
+: serializer32_backwards (serialize_x509_extensions_inner_sequence_TLV s)
+= coerce_serializer32_backwards
+  (* s2  *) (serialize_x509_extensions_inner_sequence_TLV s)
+  (* s32 *) (serialize32_asn1_sequence_TLV_backwards
+             (* ls *) (s32))
+  (* prf *) ()
+
+
+(* outmost explicit tag*)
+
+let x509_extensions_outmost_explicit_tag: asn1_tag_t
+= CUSTOM_TAG CONTEXT_SPECIFIC CONSTRUCTED 3uy
+
+let x509_extensions_t_inbound
+  (#k: parser_kind)
+  (#t: Type0)
+  (#p: parser k t)
+  (s: serializer p)
+= inbound_envelop_tag_with_value_of
+  (* tag *) x509_extensions_outmost_explicit_tag
+  (*  s  *) (serialize_x509_extensions_inner_sequence_TLV s)
+
+let parse_x509_extensions_TLV
+  (#k: parser_kind)
+  (#t: Type0)
+  (#p: parser k t)
+  (s: serializer p)
+: parser (parse_asn1_envelop_tag_with_TLV_kind x509_extensions_outmost_explicit_tag) (x509_extensions_t_inbound s)
+= x509_extensions_t_inbound s
+  `coerce_parser`
+  parse_asn1_envelop_tag_with_TLV
+  (* tag *) x509_extensions_outmost_explicit_tag
+  (*  s  *) (serialize_x509_extensions_inner_sequence_TLV s)
+
+let serialize_x509_extensions_TLV
+  (#k: parser_kind)
+  (#t: Type0)
+  (#p: parser k t)
+  (s: serializer p)
+: serializer (parse_x509_extensions_TLV s)
+= coerce_parser_serializer
+  (* p *) (parse_x509_extensions_TLV s)
+  (* s *) (serialize_asn1_envelop_tag_with_TLV
+           (* tag *) x509_extensions_outmost_explicit_tag
+           (*  s  *) (serialize_x509_extensions_inner_sequence_TLV s))
+  (*prf*) ()
+
+
+let lemma_serialize_x509_extensions_TLV_unfold
+  (#k: parser_kind)
+  (#t: Type0)
+  (#p: parser k t)
+  (s: serializer p)
+  (x: x509_extensions_t_inbound s)
+: Lemma ( predicate_serialize_asn1_sequence_TLV_unfold (serialize_x509_extensions_inner_sequence_TLV s) x )
+= lemma_serialize_asn1_sequence_TLV_unfold (serialize_x509_extensions_inner_sequence_TLV s) x
+
+let lemma_serialize_x509_extensions_TLV_size
+  (#k: parser_kind)
+  (#t: Type0)
+  (#p: parser k t)
+  (s: serializer p)
+  (x: x509_extensions_t_inbound s)
+: Lemma ( predicate_serialize_asn1_sequence_TLV_size (serialize_x509_extensions_inner_sequence_TLV s) x )
+= lemma_serialize_asn1_sequence_TLV_size (serialize_x509_extensions_inner_sequence_TLV s) x
+
+let serialize32_x509_extensions_TLV_backwards
+  (#k: parser_kind)
+  (#t: Type0)
+  (#p: parser k t)
+  (#s: serializer p)
+  (s32: serializer32_backwards s)
+: serializer32_backwards (serialize_x509_extensions_TLV s)
+= coerce_serializer32_backwards
+  (* s2  *) (serialize_x509_extensions_TLV s)
+  (* s32 *) (serialize32_asn1_envelop_tag_with_TLV_backwards
+             (* tag *) x509_extensions_outmost_explicit_tag
+             (* s32 *) (serialize32_x509_extensions_inner_sequence_TLV_backwards s32))
+  (* prf *) ()
