src/riot/x509/X509.BasicFields.fst
@@ -2,3 +2,4 @@ module X509.BasicFields
 
 include X509.BasicFields.SubjectPublicKeyInfo
 include X509.BasicFields.Extension
+include X509.BasicFields.Extensions
